src/syntax/syntax.fs
@@ -227,6 +227,8 @@ type qualifier =
   | ExceptionConstructor                   //a constructor of Prims.exn
   | HasMaskedEffect                        //a let binding that may have a top-level effect
   | Effect                                 //qualifier on a name that corresponds to an effect constructor
+  | OnlyName                               //qualifier internal to the compiler indicating a dummy declaration which
+                                           //is present only for name resolution and will be elaborated at typechecking
 
 type tycon = lident * binders * typ                   (* I (x1:t1) ... (xn:tn) : t *)
 type monad_abbrev = {
