examples/paradoxes/russell.fst
@@ -10,26 +10,26 @@ open FStar.Constructive
    by Bart Jacobs (http://people.cs.kuleuven.be/~bart.jacobs/coq-essence.pdf)
    which in turn is based on a proof by Paolo Capriotti. *)
 
-type U = | Set : i:Type  -> p:(i -> Type) -> f:(i -> Tot U) -> U
+noeq type u_type : Type u#(1 + max 'ua 'ub)= | Set : i:Type 'ua  -> p:(i -> Type 'ub) -> f:(i -> Tot u_type) -> u_type
 
-type in_set (x:U) (y:U) =
-  cexists (fun (ii:Set.i y) -> cand (Set.p y ii) (ceq (Set.f y ii) x))
+type in_set (x:u_type) (y:u_type) =
+  cexists (fun (ii:Set?.i y) -> cand (Set?.p y ii) (ceq (Set?.f y ii) x))
 
-val id : U -> Tot U
+val id : u_type -> Tot u_type
 let id x = x
 
 (* The definition of spec fails in Coq because of a universe inconsistency *)
-val spec : (U -> Type) -> Tot U
-let spec (p:(U->Type)) = Set U p id
+val spec : (u_type -> Type) -> Tot u_type
+let spec (p:(u_type->Type)) = Set u_type p id
 
-val spec_intro : p:(U->Type) -> x:U -> h:(p x) -> Tot (in_set x (spec p))
-let spec_intro (p:U->Type) (x:U) (h:(p x)) = ExIntro x (Conj h Refl)
+val spec_intro : p:(u_type->Type) -> x:u_type -> h:(p x) -> Tot (in_set x (spec p))
+let spec_intro (p:u_type->Type) (x:u_type) (h:(p x)) = ExIntro x (Conj h Refl)
 
-val spec_elim : p:(U->Type) -> x:U -> h:(in_set x (spec p)) -> Tot (p x)
-let spec_elim (p:U->Type) (x:U) h =
+val spec_elim : p:(u_type->Type) -> x:u_type -> h:(in_set x (spec p)) -> Tot (p x)
+let spec_elim (p:u_type->Type) (x:u_type) h =
   let ExIntro i (Conj h1 h2) = h in h1
 
-type pr (x:U) = cnot (in_set x x)
+type pr (x:u_type) = cnot (in_set x x)
 
 val contradiction : p:Type -> h1:(cnot p -> Tot       p ) ->
                               h2:(     p -> Tot (cnot p)) -> Tot cfalse
@@ -37,7 +37,7 @@ let contradiction (p:Type) h1 h2 =
   (fun (h3:(cnot p)) -> h3 (h1 h3)) (fun (hp:p) -> h2 hp hp)
 
 val absurd : unit -> Tot cfalse
-let absurd () = 
+let absurd () =
   let r = spec pr in
   contradiction (in_set r r)
                 (spec_intro pr r)
